Rename variables, formatting

Iris/Iris/ProofMode/Tactics/Combine.lean
@@ -68,7 +68,7 @@ theorem combine_gives_step [BI PROP] {e e1 e2 out1 out2 out : PROP}
 
 /--
   Given any Iris proposition `origE` and `goal`, the structure
-  `CombineState origE goal` consists of a collection of hypotheses
+  `CombineAsState origE goal` consists of a collection of hypotheses
   `newHyps` (representing `newE`), a Boolean value `p` and a proposition
   `out'` such that `origE` is equivalent to `newE ∗ □?p out'`.
 
@@ -79,7 +79,7 @@ theorem combine_gives_step [BI PROP] {e e1 e2 out1 out2 out : PROP}
   structure. This is necessary because one, for example, should be able to
   combine `□HP : emp` with `∗HQ : Q` to get `emp ∗ Q` instead of just `Q`.
 -/
-private structure CombineState {u} {prop : Q(Type u)} {bi} (origE goal : Q($prop)) where
+private structure CombineAsState {u} {prop : Q(Type u)} {bi} (origE goal : Q($prop)) where
   {newE : Q($prop)}
   {p : Q(Bool)}
   {out' : Q($prop)}
@@ -95,154 +95,16 @@ private def updateSt {u} {prop : Q(Type u)} {bi : Q(BI $prop)} {p1 p2 : Q(Bool)}
     (newHyps : Hyps bi e2)
     (goal : Q($prop))
     (inst : Q(CombineSepAs $out1' $out2' $out')) :
-    @CombineState u prop bi origE goal :=
+    @CombineAsState u prop bi origE goal :=
   let pf' := q(combine_as_step $pf1 $(pf2).mp $inst)
   match matchBool p1, matchBool p2 with
   | .inl _, .inl _ => { newHyps, p := q(true), out', pf1 := q($pf'), pf := q(($pf').trans)}
   | .inl _, .inr _ => { newHyps, p := q(false), out', pf1 := q($pf'), pf := q(($pf').trans)}
   | .inr _, _ => { newHyps, p := q(false), out', pf1 := q($pf'), pf := q(($pf').trans)}
 
-/-- The tactic `icombine` combines two propositions into one using the type
-    class `CombineSepAs` or, by default, the separating conjunction.
-    The Boolean value `recCall` indicates whether this function is currently
-    being called recursively. -/
-private def iCombineAsCore {u} {prop : Q(Type u)} {bi e}
-  (hyps : Hyps bi e) (goal : Q($prop)) (hs : List Ident)
-  (pat : iCasesPat) (recCall : Bool := false) :
-  ProofModeM Q($e ⊢ $goal) := do
-    match hs with
-    -- Introduce `emp` if no hypothesis is given as `icombine` arguments
-    | [] => do
-      let pf ← iCasesCore _ hyps goal pat q(true) q(emp) addBIGoal
-      return q(combine_as_nil $pf)
-
-    -- No hypothesis combined if exactly one hypothesis is given as an `icombine` argument
-    | [h1] => do
-      let ivar ← hyps.findWithInfo h1
-      -- The second argument to `hyps.remove` is set as `false`
-      let ⟨_, hyps, _, out', p, _, pf1⟩ := hyps.remove false ivar
-      let pf2 ← iCasesCore _ hyps goal pat p out' addBIGoal
-      return q(combine_as_singleton $pf1 $pf2)
-
-    -- Combine the hypotheses if two or more are given as `icombine` arguments
-    | h1 :: h2 :: htail => do
-      let ivar1 ← hyps.findWithInfo h1
-      let ivar2 ← hyps.findWithInfo h2
-
-      /- The Boolean value `recCall` indicates that `iCombineAsCore` is
-         currently is called recursively. In this case, the first hypothesis in
-         the list is temporary and should be removed even if it is in the
-         non-spatial context. -/
-      let ⟨_, hyps1, _, out1', p1, _, pf1⟩ := hyps.remove recCall ivar1
-      if (h2 :: htail).contains h1 ∧ ¬isTrue p1 then
-        throwError "icombine: propositions in the spatial context cannot be used as arguments multiple times"
-      let ⟨_, hyps2, _, out2', p2, _, pf2⟩ := hyps1.remove false ivar2
-
-      let out ← mkFreshExprMVarQ _
-      let some inst ← ProofModeM.trySynthInstanceQ q(CombineSepAs $out1' $out2' $out)
-      -- The error should not happen as the default option is always available
-      | throwError "icombine: no type class instance to combine propositions"
-
-      match htail with
-      | [] =>
-        /- Introduce the new hypothesis that combines the two original
-           hypotheses into the proof state, and generate the new proof goal for
-           the tactic user. The combined proposition is introduced into the
-           intuitionistic context if `p1` and `p2` are true. -/
-        match matchBool p1, matchBool p2 with
-        | .inl _, .inl _ =>
-          let pf3 ← iCasesCore _ hyps2 goal pat q(true) out addBIGoal
-          return q(combine_as_step $pf1 $pf2 $pf3 $inst)
-        | .inl _, .inr _ =>
-          let pf3 ← iCasesCore _ hyps2 goal pat q(false) out addBIGoal
-          return q(combine_as_step $pf1 $pf2 $pf3 $inst)
-        | .inr _, _ =>
-          let pf3 ← iCasesCore _ hyps2 goal pat q(false) out addBIGoal
-          return q(combine_as_step $pf1 $pf2 $pf3 $inst)
-      | htail =>
-        -- Create a temporary identifier for the combined hypothesis
-        let id ← mkFreshId
-        let h := mkIdent id
-
-        /- Add the combined hypothesis to the proof state and into the list
-           `hs` for the recursive function call. -/
-        match matchBool p1, matchBool p2 with
-        | .inl _, .inl _ =>
-          let newHyps := hyps2.add bi id id q(true) out
-          let pf3 ← iCombineAsCore newHyps goal (h :: htail) pat true
-          return q(combine_as_step $pf1 $pf2 $pf3 $inst)
-        | .inl _, .inr _ =>
-          let newHyps := hyps2.add bi id id q(false) out
-          let pf3 ← iCombineAsCore newHyps goal (h :: htail) pat true
-          return q(combine_as_step $pf1 $pf2 $pf3 $inst)
-        | .inr _, _ =>
-          let newHyps := hyps2.add bi id id q(false) out
-          let pf3 ← iCombineAsCore newHyps goal (h :: htail) pat true
-          return q(combine_as_step $pf1 $pf2 $pf3 $inst)
-  termination_by hs.length
-
-/-- Use the type class `CombineSepGives` to derive a new proposition in the
-    the intutitionistic context and retain the original hypotheses  -/
-private def iCombineGivesCore {u} {prop : Q(Type u)} {bi e}
-  (hyps : Hyps bi e) (goal : Q($prop)) (hs : List Ident) (pat : iCasesPat)
-  (recCall : Bool := false) :
-  ProofModeM Q($e ⊢ $goal) := do
-    match hs with
-    -- Combine the hypotheses if two or more are given as `icombine` arguments
-    | h1 :: h2 :: htail => do
-      let ivar1 ← hyps.findWithInfo h1
-      let ivar2 ← hyps.findWithInfo h2
-
-      -- USe `hyps.remove` to extract `out1` and `out2` for `CombineSepGives`
-      let ⟨e1, hyps1, out1, _, p1, _, pf1⟩ := hyps.remove recCall ivar1
-
-      if (h2 :: htail).contains h1 ∧ ¬isTrue p1 then
-        throwError "icombine: propositions in the spatial context cannot be used as arguments multiple times"
-
-      let ⟨_, _, out2, _, _, _, pf2⟩ := hyps1.remove false ivar2
-
-      let out ← mkFreshExprMVarQ _
-      let some inst ← ProofModeM.trySynthInstanceQ q(CombineSepGives $out1 $out2 $out)
-      -- Throw an error if a non-trivial fact is not found
-      | throwError "icombine: no type class instance to combine propositions"
-
-      match htail, recCall with
-      | [], true =>
-        -- Introduce the new hypothesis into the intuitionistic context and the new proof goal
-        -- Note that we use the original set of hypothesis (`hyps`)
-        let pf3 ← iCasesCore _ hyps1 goal pat q(true) out addBIGoal
-
-        match matchBool p1 with
-        | .inl _ =>
-          let pf4 := q($(pf1).mp.trans sep_elim_l)
-          return q(combine_step_gives $pf1 $pf2 $pf3 $pf4 $inst)
-        | .inr _ =>
-          -- This should never happen as the intermediate proposition generated
-          -- by `iCombineGivesCore` exists in the intuitionistic context
-          throwAbortTactic
-      | [], false =>
-        let pf3 ← iCasesCore _ hyps goal pat q(true) out addBIGoal
-        return q(combine_step_gives $pf1 $pf2 $pf3 refl $inst)
-      | htail, _ =>
-        -- Create a temporary identifier for the combined hypothesis
-        let id ← mkFreshId
-        let h := mkIdent id
-
-        let newHyps := hyps.add bi id id q(true) out
-        let pf3 ← iCombineGivesCore newHyps goal (h :: htail) pat true
-
-        return q(combine_step_gives $pf1 $pf2 $pf3 refl $inst)
-    | _ => do
-      -- Introduce `True` if less than two hypotheses are given as an `icombine` argument
-      let pf ← iCasesCore _ hyps goal pat q(true) q(iprop(True)) addBIGoal
-      return q(combine_nil_singleton_gives $pf)
-  termination_by hs.length
-
-theorem dummy [BI PROP] {a b c : PROP} : a ⊢ b ∗ c := sorry
-
-private def CombineState.combineAsProofModeHyp {u prop bi origE goal} :
-    @CombineState u prop bi origE goal → IVarId  →
-    ProofModeM (@CombineState u prop bi origE goal)
+private def CombineAsState.combineAsProofModeHyp {u prop bi origE goal} :
+    @CombineAsState u prop bi origE goal → IVarId  →
+    ProofModeM (@CombineAsState u prop bi origE goal)
   | { newE, newHyps, p, out', pf1, init .. }, ivar => do
       let ⟨e2, hyps2, _, out2', p2, _, pf2⟩ := newHyps.remove false ivar
       match matchBool p, out', matchBool init with
@@ -275,10 +137,8 @@ private def CombineGivesState.combineGivesProofModeHyp {u prop bi e goal} :
       let newOut ← mkFreshExprMVarQ _
       let some inst ← ProofModeM.trySynthInstanceQ q(CombineSepGives iprop(□ $out') $out2 $newOut)
       | throwError "icombine: no type class instance to combine propositions"
-
       let pf1 : Q($e ⊢ $e ∗ □ $newOut) := q(combine_gives_step ⟨$pf1, sep_elim_l⟩ $pf2 $inst)
       let pf : Q(($e ∗ □ $newOut ⊢ $goal) → ($e ⊢ $goal)) := q($(pf1).trans)
-
       return { hyps, out' := newOut, pf1, pf }
 
 /-- The tactic `icombine` combines propositions into one using the type
@@ -290,8 +150,8 @@ elab "icombine" idents:(colGt ident)* "as" colGt patAs:icasesPat : tactic => do
   ProofModeM.runTactic λ mvar { e, hyps, goal, .. } => do
     let hs := idents.toList
 
-    -- Initialise a mutable instance of `CombineState`
-    let mut st : CombineState e goal := {
+    -- Initialise a mutable instance of `CombineAsState`
+    let mut st : CombineAsState e goal := {
       -- Nothing is part of the combined hypothesis initially
       newE := q($e),
       newHyps := hyps,
@@ -308,11 +168,9 @@ elab "icombine" idents:(colGt ident)* "as" colGt patAs:icasesPat : tactic => do
     for h in hs do
       -- Find the `IVarId` of the hypothesis
       let ivar ← hyps.findWithInfo h
-
       -- Hypothesis in the spatial context should not be used multiple times
       if hs.count h > 1 ∧ ¬isTrue (← hyps.findP h) then
         throwError "icombine: propositions in the spatial context cannot be used as arguments multiple times"
-
       st ← st.combineAsProofModeHyp ivar
 
     -- Generate the new proof goal for the user and fill in the metavariable
@@ -365,7 +223,6 @@ elab "icombine" idents:(colGt ident)* "gives" colGt patGives:icasesPat : tactic 
       -- Generate the new proof goal for the user and fill in the metavariable
       let pf' ← iCasesCore _ st.hyps goal pat q(true) st.out' addBIGoal
       mvar.assign q($(st.pf) $pf')
-
     | _ =>
       -- Introduce `True` into the intuitionistic context if less than two hypotheses are given
       let pf' ← iCasesCore _ hyps goal pat q(true) q(iprop(True)) addBIGoal
